theories/Pipeline.v
@@ -10,7 +10,8 @@ From MetaRocq.Erasure Require EAstUtils ErasureFunction ErasureCorrectness EImpl
 From MetaRocq Require Import ETransform EConstructorsAsBlocks.
 From MetaRocq.Erasure Require Import EWcbvEvalNamed.
 From MetaRocq.ErasurePlugin Require Import Erasure ErasureCorrectness.
-From Malfunction Require Import CeresSerialize CompileCorrect SemanticsSpec FFI.
+From Malfunction Require Import CompileCorrect SemanticsSpec FFI.
+From Ceres Require Import CeresSerialize.
 Import PCUICProgram.
 (* Import TemplateProgram (template_eta_expand).
  *)
@@ -29,10 +30,10 @@ Proof using Type.
   - repeat econstructor.
   - sq. now constructor.
 Qed.
-  
+
 Import Transform.Transform.
 
-#[local] Arguments transform : simpl never. 
+#[local] Arguments transform : simpl never.
 
 #[local] Obligation Tactic := program_simpl.
 
@@ -44,8 +45,8 @@ Import EWcbvEval.
 
 From Malfunction Require Import Compile Serialize.
 
-Record malfunction_pipeline_config := 
-  { erasure_config :> erasure_configuration; 
+Record malfunction_pipeline_config :=
+  { erasure_config :> erasure_configuration;
     reorder_cstrs : EProgram.inductives_mapping;
     prims : Malfunction.primitives }.
 
@@ -54,7 +55,7 @@ Definition int_to_nat (i : Uint63.int) : nat :=
 
 Definition array_length := Eval cbv in PArray.max_length.
 
-Record good_for_extraction (fl : EWellformed.EEnvFlags) (p : program (list (kername × EAst.global_decl)) EAst.term) := 
+Record good_for_extraction (fl : EWellformed.EEnvFlags) (p : program (list (kername × EAst.global_decl)) EAst.term) :=
   {
     few_enough_blocks :
       forall (i : inductive) (args : list nat), lookup_constructor_args p.1 i = Some args -> blocks_until #|args| args < 200 ;
@@ -99,7 +100,7 @@ Section params.
   Fixpoint wellformed_fast (t : EAst.term) {struct t} : bool :=
     match t with
     | EAst.tBox => EWellformed.has_tBox
-    | EAst.tRel i => EWellformed.has_tRel 
+    | EAst.tRel i => EWellformed.has_tRel
     | EAst.tVar _ => EWellformed.has_tVar
     | EAst.tEvar _ args => EWellformed.has_tEvar && forallb (wellformed_fast) args
     | EAst.tLambda _ M => EWellformed.has_tLambda && wellformed_fast M
@@ -108,7 +109,7 @@ Section params.
     | EAst.tConst kn =>
         EWellformed.has_tConst
     | EAst.tConstruct ind c block_args =>
-        EWellformed.has_tConstruct 
+        EWellformed.has_tConstruct
     | EAst.tCase ind c brs =>
         EWellformed.has_tCase &&
           (let brs' := forallb (fun br : list BasicAst.name × EAst.term => wellformed_fast  br.2) brs in
@@ -127,7 +128,7 @@ Fixpoint check_good_for_extraction_rec (fl : EWellformed.EEnvFlags) (Σ : (list 
   | nil => true
   | (kn, EAst.ConstantDecl d) :: Σ =>
       match (EAst.cst_body d) with
-      | Some b => if wellformed_fast fl Σ b 
+      | Some b => if wellformed_fast fl Σ b
                   then check_good_for_extraction_rec fl Σ
                   else ignore (coq_msg_info "Warning: environment contains constructors for which extraction is not verified") (check_good_for_extraction_rec fl Σ)
       | None => ignore (coq_msg_info ("Warning: environment contains axiom " ++ Kernames.string_of_kername kn)) false
@@ -144,7 +145,7 @@ Fixpoint check_good_for_extraction_rec (fl : EWellformed.EEnvFlags) (Σ : (list 
   end.
 
 Definition check_good_for_extraction fl (p : program (list (kername × EAst.global_decl)) EAst.term) :=
-  if wellformed_fast fl p.1 p.2 then 
+  if wellformed_fast fl p.1 p.2 then
     check_good_for_extraction_rec fl p.1
   else ignore (coq_msg_info "Warning: term contains constructors for which extraction is not verified") (check_good_for_extraction_rec fl p.1).
 
@@ -165,7 +166,7 @@ Definition extraction_term_flags_mlf :=
     EWellformed.has_tProj := false;
     EWellformed.has_tFix := true;
     EWellformed.has_tCoFix := false;
-    EWellformed.has_tPrim := 
+    EWellformed.has_tPrim :=
       {| EWellformed.has_primint := true;
          EWellformed.has_primfloat := true;
          EWellformed.has_primstring := false;
@@ -191,7 +192,7 @@ Program Definition enforce_extraction_conditions `{Pointer} `{Heap} :
     (EProgram.eval_eprogram block_wcbv_flags) (EProgram.eval_eprogram block_wcbv_flags) :=
   {|
     name := "Enforce the term is extractable" ;
-    transform p _ := 
+    transform p _ :=
       let r := check_good_for_extraction extraction_env_flags_mlf p in
       ignore r p ;
     (* if check_good_for_extraction extraction_env_flags_mlf p then p else p ; *)
@@ -285,7 +286,7 @@ Proof.
   rewrite !lookup_env_annotate.
   destruct EGlobalEnv.lookup_env; try reflexivity.
   cbn.
-  destruct g; cbn; try reflexivity. 
+  destruct g; cbn; try reflexivity.
   destruct c; cbn; try reflexivity.
   destruct cst_body0; reflexivity.
 Qed.
@@ -329,7 +330,7 @@ Proof.
     clear H1. cbn in *. clear H. induction Σ; cbn.
   - econstructor.
   - destruct a. destruct g. destruct c. destruct cst_body0.
-    * invs H0. constructor; eauto. 
+    * invs H0. constructor; eauto.
       cbn in *. now eapply (wellformed_annotate' _ _ [] []) in H4.
       cbn in *. now eapply annotate_env_fresh.
     * invs H0. econstructor; eauto.
@@ -344,11 +345,11 @@ Program Definition name_annotation : Transform.t EAst.global_declarations (list 
   EAst.term EAst.term _ EWcbvEvalNamed.value
   (EProgram.eval_eprogram extraction_wcbv_flags) (fun p v => ∥EWcbvEvalNamed.eval p.1 [] p.2 v∥) :=
   {| name := "annotate names";
-      pre := fun p =>  good_for_extraction (switch_off_box extraction_env_flags_mlf) p /\ 
+      pre := fun p =>  good_for_extraction (switch_off_box extraction_env_flags_mlf) p /\
         EProgram.wf_eprogram (switch_off_box extraction_env_flags_mlf) p ;
       transform p _ := (annotate_env [] p.1, annotate [] p.2) ;
       post := fun p => good_for_extraction named_extraction_env_flags_mlf p /\
-                      exists t, wellformed (switch_off_box extraction_env_flags_mlf) p.1 0 t 
+                      exists t, wellformed (switch_off_box extraction_env_flags_mlf) p.1 0 t
                       /\ ∥represents [] [] p.2 t∥ ;
       obseq p _ p' v v' := ∥ represents_value v' v∥ |}.
 Next Obligation.
@@ -359,23 +360,23 @@ Next Obligation.
   cbn in *. split.
   2:{ sq. eapply (nclosed_represents (switch_off_box extraction_env_flags_mlf)); cbn; eauto. }
   clear - Hs. revert Hs. generalize 0. intros.
-  induction s using EInduction.term_forall_list_ind in n, Hs |- *; cbn in *; eauto; rtoProp; eauto. 
-  all: try now rtoProp; eauto. 
+  induction s using EInduction.term_forall_list_ind in n, Hs |- *; cbn in *; eauto; rtoProp; eauto.
+  all: try now rtoProp; eauto.
   - unfold EGlobalEnv.lookup_constant in *. rewrite lookup_env_annotate. destruct EGlobalEnv.lookup_env as [ [[ [] ] | ] | ]; cbn in *; eauto.
-  - unfold EGlobalEnv.lookup_constructor_pars_args, EGlobalEnv.lookup_constructor, EGlobalEnv.lookup_inductive, EGlobalEnv.lookup_minductive in *. rewrite lookup_env_annotate. 
+  - unfold EGlobalEnv.lookup_constructor_pars_args, EGlobalEnv.lookup_constructor, EGlobalEnv.lookup_inductive, EGlobalEnv.lookup_minductive in *. rewrite lookup_env_annotate.
     destruct EGlobalEnv.lookup_env as [ [[ [] ] | ] | ]; cbn in *; eauto.
     destruct nth_error; cbn in *; try congruence.
     destruct nth_error; cbn in *; try congruence.
     repeat split; eauto.
     solve_all.
   - revert H; unfold wf_brs. unfold EGlobalEnv.lookup_inductive, EGlobalEnv.lookup_minductive in *.
-    rewrite lookup_env_annotate. 
+    rewrite lookup_env_annotate.
     destruct EGlobalEnv.lookup_env as [ [[ [] ] | ] | ]; cbn in *; eauto.
-    destruct nth_error; cbn in *; try congruence.  
+    destruct nth_error; cbn in *; try congruence.
     repeat split; eauto.
     solve_all.
   - solve_all. unfold wf_fix in *. rtoProp. solve_all.
-  - solve_all. destruct p as [? []]; cbn in *; eauto. 
+  - solve_all. destruct p as [? []]; cbn in *; eauto.
 Qed.
 Next Obligation.
   red. intros. destruct pr as [_ pr]. red in H. sq.
@@ -399,7 +400,7 @@ Next Obligation.
       2-4: eapply IHg; now invs H0.
       split; eauto. eexists. split. cbn. reflexivity.
       eapply (nclosed_represents (switch_off_box extraction_env_flags_mlf)); cbn => //. invs H0. cbn in *. eauto.
-  - eapply pr.  
+  - eapply pr.
 Qed.
 
 Lemma annotate_extends (efl := switch_off_box extraction_env_flags_mlf) Σ Σ' :
@@ -407,7 +408,7 @@ Lemma annotate_extends (efl := switch_off_box extraction_env_flags_mlf) Σ Σ' :
    EGlobalEnv.extends (annotate_env [] Σ) (annotate_env [] Σ').
 Proof.
   red. intros ext kn decl Hdecl. rewrite lookup_env_annotate in Hdecl.
-  rewrite lookup_env_annotate. eapply option_map_Some in Hdecl as [? [? ?]]. 
+  rewrite lookup_env_annotate. eapply option_map_Some in Hdecl as [? [? ?]].
   erewrite ext; cbn; eauto. now f_equal.
 Qed.
 
@@ -425,16 +426,16 @@ Program Definition compile_to_malfunction `{Heap}:
 Next Obligation. sq.
   erewrite (map_ext _ fst).
   eapply (compile_wellformed _ 0 _ H2).
-  eapply H3. 
+  eapply H3.
   eapply H4. eapply H5.
   intros. now destruct x.
 Qed.
 Next Obligation.
-  red. intros. exists (compile_value p.1 v); eauto. 
+  red. intros. exists (compile_value p.1 v); eauto.
 Qed.
 
 Program Definition post_verified_named_erasure_pipeline `{Heap}:
- Transform.t EAst.global_declarations _ _ _ _ EWcbvEvalNamed.value  
+ Transform.t EAst.global_declarations _ _ _ _ EWcbvEvalNamed.value
  (eval_eprogram EConstructorsAsBlocks.block_wcbv_flags)
  (fun p v => ∥ EWcbvEvalNamed.eval p.1 [] p.2 v ∥)  :=
   enforce_extraction_conditions ▷
@@ -442,14 +443,14 @@ Program Definition post_verified_named_erasure_pipeline `{Heap}:
   name_annotation.
 
 Program Definition verified_named_erasure_pipeline `{Heap}:
- Transform.t global_env_ext_map _ _ _ _ EWcbvEvalNamed.value 
+ Transform.t global_env_ext_map _ _ _ _ EWcbvEvalNamed.value
              PCUICTransform.eval_pcuic_program
              (fun p v => ∥ EWcbvEvalNamed.eval p.1 [] p.2 v ∥) :=
   verified_erasure_pipeline ▷
   post_verified_named_erasure_pipeline.
 
 Program Definition verified_malfunction_pipeline `{Heap} :
- Transform.t global_env_ext_map _ _ _ _ SemanticsSpec.value 
+ Transform.t global_env_ext_map _ _ _ _ SemanticsSpec.value
              PCUICTransform.eval_pcuic_program
              (fun _ _ => True) :=
   verified_named_erasure_pipeline ▷
@@ -457,7 +458,7 @@ Program Definition verified_malfunction_pipeline `{Heap} :
 Next Obligation.
   cbn. intros.
   destruct p as [Σ t]. split. apply H1. sq. split. 2: eauto.
-  eexists. split. 2:sq. all:eauto. 
+  eexists. split. 2:sq. all:eauto.
 Qed.
 
 Section compile_malfunction_pipeline.
@@ -477,8 +478,8 @@ Section compile_malfunction_pipeline.
   Variable Normalisation : forall Σ0 : global_env_ext, wf_ext Σ0 -> NormalizationIn Σ0.
 
   Definition compile_malfunction_pipeline := transform verified_malfunction_pipeline (Σ, t) (precond _ _ _ _ expΣ expt typing _).
-  
-End compile_malfunction_pipeline. 
+
+End compile_malfunction_pipeline.
 
 Arguments compile_malfunction_pipeline {_ _ _ _ _ _} _ _ _ {_}.
 
@@ -502,13 +503,13 @@ Proof.
   destruct enable_unsafe as [[] ? ? ?] => //.
 Qed.
 
-Program Definition malfunction_pipeline 
+Program Definition malfunction_pipeline
   (config : malfunction_pipeline_config) :
   Transform.t _ _ _ _ _ _ eval_template_program_mapping
              (fun _ _ => True) :=
-  pre_erasure_pipeline_mapping ▷ 
-  switchable_erasure_pipeline config ▷ 
-  post_verified_named_erasure_pipeline ▷ 
+  pre_erasure_pipeline_mapping ▷
+  switchable_erasure_pipeline config ▷
+  post_verified_named_erasure_pipeline ▷
   compile_to_malfunction.
 Next Obligation.
   unfold switchable_erasure_pipeline.
@@ -537,6 +538,5 @@ Definition compile_malfunction_gen config (pt : program_type) (p : Ast.Env.progr
 Definition default_malfunction_config : malfunction_pipeline_config :=
   {| erasure_config := safe_erasure_config; reorder_cstrs := []; prims := [] |}.
 
-Definition compile_malfunction p := 
+Definition compile_malfunction p :=
   (compile_malfunction_gen default_malfunction_config Standalone p).2.
-
